LeanProjeto2/Basic.lean
@@ -1,2 +1,5 @@
 def hello := "world"
 #eval hello
+
+
+-- importar o StarLang
