LeanProjeto2/SHFunctInterp.lean
@@ -1,0 +1,228 @@
+-- -------------------------------------------------------------
+--          SHOENFIELD'S FUNCTIONAL INTERPRETATION
+-- -------------------------------------------------------------
+
+import LeanProjeto2.FOLanguage
+import LeanProjeto2.StarLanguage.FiniteTypes
+import LeanProjeto2.StarLanguage.Syntax
+import LeanProjeto2.StarLanguage.Axioms
+import LeanProjeto2.StarLanguage.ResultsAndOtherDefinitions
+import MathLib.Tactic
+import Mathlib.Data.Finset.Basic
+import Mathlib.Data.Multiset.Basic
+
+
+open FOLang
+open LFormula
+open Term
+open Formula
+open Batteries
+
+-- SHOENFIELD'S FUNCTIONAL INTERPREATION
+
+-- ---------------------------------------------------------------------------------------------------------------
+--             SECTION 2.2: Shoenfield's functional interpretation
+-- ---------------------------------------------------------------------------------------------------------------
+
+-- -------------------------------------------------------------
+-- DEFINITION 2.1 (p.38): Shoenfield's functional interpretation
+-- -------------------------------------------------------------
+
+/-
+To define Shoenfield's functional interpretation we need some auxiliary functions to deal with the
+different components of the interpretation of a formula. Every interpretation has a list of universal
+variables, a list of existential variables and the matrix, i.e. the lower SH-formula (a base formula).
+These three components will be represented by a tuple.
+
+For example, if a formula A has the interpretation A^SH given by
+                        ∀a ∃b A_SH(a,b)
+then we would represent this as (a,b,A_SH).
+
+The function 'components' transforms a formula such as ∀a ∃b A_SH(a,b) into the tupe (a,b,A_SH).
+The function 'Recreate' transforms a tuple such as (a,b,A_SH) into the formula ∀a ∃b A_SH(a,b).
+-/
+
+-- É PRECISO ACRESCENTAR ISFULLYBASE, aka que temos necessariamente uma fórmula sem ∀ e sem ∃ na matriz
+
+#check isBase
+
+def Formula.components : Formula → (Finset String × Finset String × Formula)
+| unbForall x A =>
+    let (a, b, rest) := A.components
+    ({x} ∪ a, b, rest)
+| not (unbForall x A) =>
+    let (a, b, rest) := A.components
+    (a, {x} ∪ b, rest)
+| not A =>
+    let (a, b, rest) := A.components
+    (a, b, not rest)
+--| bForall x t A =>
+--    let (a, b, rest) := A.components
+--    (a, {x} ∪ b, bForall x t rest)
+| or A1 A2 =>
+    let (a1, b1, r1) := A1.components
+    let (a2, b2, r2) := A2.components
+    (a1 ∪ a2, b1 ∪ b2, or r1 r2)
+| A => ({}, {}, A)
+-- Reunião: daria se calhar para pôr aqui um not e forall
+-- Só se pode usar quando ja estiver com ∀a ∃b
+
+def Formula.components2 : Formula → (List String × List String × Formula)
+| unbForall x A =>
+    let (a, b, rest) := A.components2
+    ({x} ∪ a, b, rest)
+| not (unbForall x A) =>
+    let (a, b, rest) := A.components2
+    (a, {x} ∪ b, rest)
+| not A =>
+    let (a, b, rest) := A.components2
+    (a, b, not rest)
+--| bForall x t A =>
+--    let (a, b, rest) := A.components
+--    (a, {x} ∪ b, bForall x t rest)
+| or A1 A2 =>
+    let (a1, b1, r1) := A1.components2
+    let (a2, b2, r2) := A2.components2
+    (a1 ∪ a2, b1 ∪ b2, or r1 r2)
+| A => ({}, {}, A)
+
+
+-- -------
+-- Example to use components:
+-- -------
+
+def formula_teste (A:Formula) : Formula := (∀₁₁ "x" (∃₁₁ "y" (∃₁₁ "z" (¬₁A))))
+#eval (formula_teste (Formula.rel "R" [var_x,var_y])).components      -- Output: ({x}, {y, z}, ¬₁R(x,y)) --> CAN I ADD SIMP??
+#eval components (∀₁₁ "x" (¬₁(∀₁₁ "y" (rel "P" [var_x, var_y]))))     -- Output: ({x}, {y, z}, ¬₁R(x,y))
+#eval components (∀₁₁ "x" ((∃₁₁ "y" (¬₁(rel "P" [var_x, var_y])))))   -- Output: ({x}, {y, z}, ¬₁R(x,y))
+
+def exampleFormula : Formula :=
+  b∀₁₁ "x" (Term.var "t") (¬₁ (∀₁₁ "y" (Formula.rel "R" [])))
+#eval exampleFormula.components       -- Output dá ({}, {x,y}, ∀x∈t R[]) --> WRONG
+
+
+noncomputable def Recreate : (Finset String × Finset String × Formula) → Formula
+| (a, b, rest) => -- Assim já ficamos com (x,y,F)
+  -- Negações dentro do b
+                let neg := List.foldl (fun f x => .unbForall x (.not f)) rest (b.val.toList : List String)
+  -- unbForall dentro do a
+                List.foldl (fun f x => .unbForall x f) neg (a.val.toList : List String)
+-- TBD (Reunião): dá para acrescentar aqui que rest is always base?
+--   -> Não vai ser consequência direta de acrescentar isBase como hipotese em components?
+
+noncomputable def Recreate2 : (List String × List String × Formula) → Formula
+| (a, b, rest) =>
+  -- Negações dentro do b
+  let neg := List.foldl (fun f x => .unbForall x (.not f)) rest b
+  -- unbForall dentro do a
+  List.foldl (fun f x => Formula.unbForall x f) neg a
+
+
+-- --------------------------------------
+-- DEFINITION 2.1 (p.38):
+-- Shoenfield's functional interpretation
+-- --------------------------------------
+
+/-
+Here we will represent an interpretation A^SH such as ∀a∃b A_SH(a,b) as
+                  ( SH_int A^SH ( Recreate (a,b,A_SH) ) )
+              ( SH_int upperSH ( Recreate (univ_var,exist_var,lowerSH) ) )
+-/
+
+
+-- TBD (Reunião): variaveis disjuntas -> Finset já tem disjunto
+--                make List α to Finset -> List.toFinset _
+-- a∪b∪c∪d : Finset     -> ver Disjoint a b c d
+inductive SH_int : Formula → Formula → Prop
+| base : (h : isFullyBase A) → (SH_int A (Recreate ({},{},A)))
+| disj : SH_int A AuSH →
+         SH_int B BuSH →
+         AuSH.components = (a,b,A_SH) →                                     -- A^SH = ∀a ∃b A_SH(a,b)
+         BuSH.components = (c,d,B_SH) →                                     -- B^SH = ∀c ∃d B_SH(c,d)
+         --({a,b} ⊆ A.allvars) →                                            -- TO DO: precisamos?
+         --({c,d} ⊆ B.allvars) →                                            -- TO DO: dizer lista não tem conjuntos repetidos
+         (hA : isFullyBase A_SH) →
+         (hB : isFullyBase B_SH) →
+         (SH_int (A∨₁B) (Recreate (a∪c,b∪d,(A_SH ∨₁ B_SH))))                -- (A∨B)^SH = ∀a,c ∃b,d [ A_SH(a,b) ∨ B_SH(c,d) ]
+| neg {f a':String}:
+        -- ({a,b} ⊆ A.allvars) →
+        SH_int A AuSH →
+        AuSH.components = (a,b,A_SH) →                                     -- A^SH = ∀a ∃b A_SH(a,b)
+        (hA : isFullyBase A_SH) →
+        (SH_int (¬₁A) (Recreate (b,b,A_SH)))--(TermTupleApp (makeTuple [Term.var f]) a)))) --→  -- TODO: apagar porque foi batota
+        --(SH_int (¬₁A) (Recreate ({f},{a'},(b∃₁ a.toList (Term.var a') (¬₁(substitution_formula b.toList ((Term.var f)·(Term.var a)) A_SH))))))
+        --(SH_int (¬₁A) (Recreate ({f},{a'},(b∃₁ a.toList (Term.var a') A))))
+        --(SH_int (¬₁A) (Recreate ({f},{a'},(b∃₁ a.toList (Term.var a') (¬₁(substitution_formula b.toList ((Term.var f)·(Term.var a)) A_SH))))))      -- TO DO / Problema: problema: o bE₁ devia então aceitar Finset String :'(
+        --((SH_int (¬₁A) (V₁ f (E₁ a' (bE₁ a (Term.var (a')) (¬₁(substitution_formula b ((Term.var f)·(Term.var a)) A_SH)))))))         -- (¬A)^SH = ∀f ∃a' [ ∃a∈a' ¬A_SH(a,fa) ]
+| unbForall : SH_int A AuSH →
+              AuSH.components = (a,b,A_SH) →                                -- A^SH = ∀a ∃b A_SH(a,b)
+              --({x,a,b} ⊆ A.allvars) →
+              --(SH_int A (V₁ a (E₁ b A_SH))) →                             -- A^SH = ∀a ∃b A_SH(a,b)
+              (hA : isFullyBase A_SH) →
+              (SH_int (∀₁₁ x A) (Recreate (a∪{x},b,A_SH)))                  -- (∀x A)^SH = ∀x,a ∃b [ A_SH(x,a,b) ]
+| bForall : SH_int A AuSH →
+            AuSH.components = (a,b,A_SH) →                                  -- A^SH = ∀a ∃b A_SH(a,b)
+            (hA : isFullyBase A_SH) →
+            (SH_int (b∀₁ x t A) (Recreate (a,b,(b∀₁ x t A_SH))))            -- (∀x∈t A(x))^SH = ∀a ∃b [ ∀x∈t A_SH(x,a,b) ]
+            --({x,a,b} ⊆ A.allvars) →
+            --(h : x ∉ t.freevars)
+
+-- TO DO (eu): a tirar este Teste e fazer um melhor
+def Teste (a b : String) (f : Term) (A_SH : Formula): Formula := substitution_formula b (f·(Term.var a)) A_SH
+
+example (A:Formula) (H : isBase A) : isBase (b∃₁₁ x t A) := by
+  exact bExists_base x t H
+
+
+inductive SH_int2 : Formula → Formula → Prop
+| base : (h : isFullyBase A) → (SH_int2 A (Recreate ({},{},A)))
+| disj : SH_int2 A AuSH →
+         SH_int2 B BuSH →
+         AuSH.components2 = (a,b,A_SH) →                                     -- A^SH = ∀a ∃b A_SH(a,b)
+         BuSH.components2 = (c,d,B_SH) →                                     -- B^SH = ∀c ∃d B_SH(c,d)
+         --({a,b} ⊆ A.allvars) →                                            -- TO DO: precisamos?
+         --({c,d} ⊆ B.allvars) →                                            -- TO DO: dizer lista não tem conjuntos repetidos
+         (hA : isFullyBase A_SH) →
+         (hB : isFullyBase B_SH) →
+         (SH_int2 (A∨₁B) (Recreate2 (a∪c,b∪d,(A_SH ∨₁ B_SH))))                -- (A∨B)^SH = ∀a,c ∃b,d [ A_SH(a,b) ∨ B_SH(c,d) ]
+| neg {f a': List String}:
+        -- ({a,b} ⊆ A.allvars) →
+        SH_int2 A AuSH →
+        (a,b,A_SH) = AuSH.components2 →                                    -- A^SH = ∀a ∃b A_SH(a,b)
+        (hA : isFullyBase A_SH) →
+        --(SH_int2 (¬₁A) (Recreate2 (b,b,(bForallTuple2 a (ls_lt a') A_SH))))--(TermTupleApp (makeTuple [Term.var f]) a)))) --→  -- TODO: apagar porque foi batota
+        --(SH_int2 (¬₁A) (Recreate2 (f,a',(b∃₁ a (Term.var a') A_SH))))
+        (SH_int2 (¬₁A) (Recreate2 (f,a',(bForallTuple2 a (ls_lt a') (¬₁(A_SH.subst (HashMap.ofList  (b.zip ((f.tt)⊙(a.tt))))))))))
+        --(SH_int (¬₁A) (Recreate ({f},{a'},(b∃₁ a.toList (Term.var a') A))))
+        --(SH_int (¬₁A) (Recreate ({f},{a'},(b∃₁ a.toList (Term.var a') (¬₁(substitution_formula b.toList ((Term.var f)·(Term.var a)) A_SH))))))      -- TO DO / Problema: problema: o bE₁ devia então aceitar Finset String :'(
+        --((SH_int (¬₁A) (V₁ f (E₁ a' (bE₁ a (Term.var (a')) (¬₁(substitution_formula b ((Term.var f)·(Term.var a)) A_SH)))))))         -- (¬A)^SH = ∀f ∃a' [ ∃a∈a' ¬A_SH(a,fa) ]
+| unbForall : SH_int2 A AuSH →
+              AuSH.components2 = (a,b,A_SH) →                                -- A^SH = ∀a ∃b A_SH(a,b)
+              --({x,a,b} ⊆ A.allvars) →
+              --(SH_int A (V₁ a (E₁ b A_SH))) →                             -- A^SH = ∀a ∃b A_SH(a,b)
+              (hA : isFullyBase A_SH) →
+              (SH_int2 (∀₁₁ x A) (Recreate2 (a∪{x},b,A_SH)))                  -- (∀x A)^SH = ∀x,a ∃b [ A_SH(x,a,b) ]
+| bForall : SH_int2 A AuSH →
+            AuSH.components2 = (a,b,A_SH) →                                  -- A^SH = ∀a ∃b A_SH(a,b)
+            (hA : isFullyBase A_SH) →
+            (SH_int2 (b∀₁ x t A) (Recreate2 (a,b,(b∀₁ x t A_SH))))            -- (∀x∈t A(x))^SH = ∀a ∃b [ ∀x∈t A_SH(x,a,b) ]
+            --({x,a,b} ⊆ A.allvars) →
+            --(h : x ∉ t.freevars)
+
+
+
+
+
+
+
+
+
+/- Next tarefas:
+    1. Pôr namespaces para os exemplos:
+        a) No FOLanguage
+        b) Axioms / FiniteTypes / Syntax / ResultsAndOtherDefinitions
+    2. Resolver isBase como hipotese em components... done?
+    3. Resolver Term.application para tuples -> Notation 1.4
+
+axiom Bla (A:Formula) : (¬₁(¬₁ A))=A
+-/
