LeanProjeto2/StarLanguage/ResultsAndOtherDefinitions.lean
@@ -11,3 +11,19 @@ import MathLib.Tactic
 
 open FOLang
 open LFormula
+
+#check 5
+#check 5+3
+
+def AddThree (n:ℕ) : ℕ := n+3
+#eval AddThree 5
+
+lemma AddResult (m n l : ℕ) : m+(n+l) = l+(n+m) :=
+  by
+    rw [← add_assoc m n l]
+    rw [add_comm (m+n) l]
+    rw [add_comm m n]
+
+lemma AddResult2 (m n l : ℕ) : m+(n+l) = l+(n+m) :=
+  by
+    linarith
